Intermediate/Composition.v
@@ -1,0 +1,393 @@
+Require Import Common.Definitions.
+Require Import Common.Util.
+Require Import Common.Memory.
+Require Import Common.Linking.
+Require Import CompCert.Events.
+Require Import CompCert.Smallstep.
+Require Import CompCert.Behaviors.
+Require Import Intermediate.Machine.
+Require Import Intermediate.GlobalEnv.
+Require Import Intermediate.CS.
+Require Import Intermediate.PS.
+Require Import Intermediate.Decomposition.
+
+Import GlobalEnv.
+Import Intermediate.
+
+Section PS2CS.
+  Variable prog: program.
+
+  Hypothesis prog_is_closed:
+    closed_program prog.
+
+  Let ctx := PMap.empty Component.interface.
+  Let G := init_genv prog.
+
+  Lemma match_initial_states:
+    forall ips,
+      PS.initial_state prog ctx ips ->
+    exists ics,
+      CS.initial_state prog ics /\ PS.partial_state ctx ics ips.
+  Proof.
+    intros ips Hips_init.
+    inversion Hips_init; subst.
+    exists ics. split; auto.
+  Qed.
+
+  Lemma match_final_states:
+    forall ips ics,
+      PS.partial_state ctx ics ips ->
+      PS.final_state prog ctx ips ->
+      CS.final_state G ics.
+  Proof.
+    intros ips ics Hics_partial Hips_final.
+    inversion Hips_final; subst.
+    (* program has control *)
+    - inversion Hics_partial; subst;
+        try (PS.simplify_turn; contradiction).
+      inversion H0; subst; try (PS.simplify_turn; contradiction).
+      inversion H11; subst; try (PS.simplify_turn; contradiction).
+      auto.
+    (* context has control *)
+    (* (contra, context is empty) *)
+    - PS.simplify_turn.
+      destruct ips.
+      + repeat destruct p.
+        exfalso.
+        eapply PMapFacts.empty_in_iff; eauto.
+      + destruct c. destruct p.
+        exfalso.
+        eapply PMapFacts.empty_in_iff; eauto.
+  Qed.
+
+  Lemma lockstep_simulation:
+    forall ips t ips',
+      PS.step ctx G ips t ips' ->
+    forall ics,
+      PS.partial_state ctx ics ips ->
+    exists ics',
+      CS.step G ics t ics' /\ PS.partial_state ctx ics' ips'.
+  Proof.
+    intros ips t ips' Hstep ics Hics_partial.
+
+    inversion Hics_partial; subst; PS.simplify_turn;
+      try (eapply PMapFacts.empty_in_iff in H; inversion H).
+
+    inversion Hstep; subst.
+
+    inversion H2; subst; PS.simplify_turn;
+      try contradiction.
+    inversion H11; subst.
+
+    assert (CS.state_eq (gps0, mem0, regs, pc) (gps, mem, regs, pc)). {
+      constructor; try reflexivity.
+      - rewrite (PS.to_partial_stack_with_empty_context gps gps0); auto.
+      - rewrite H0 in H10.
+        unfold PMap.Equal, PMapExtra.filter in *.
+        intros C. specialize (H10 C).
+        rewrite PMapExtra.fold_identity in H10.
+        rewrite PMapExtra.fold_identity in H10.
+        auto.
+    }
+
+    destruct (CS.equal_states_step G (gps0, mem0, regs, pc) t ics'
+                                   (gps, mem, regs, pc) H4 H1) as [ics'' [Hstep' Heq']].
+    eexists ics''.
+    split; auto.
+    eapply PS.equal_states_partialize; eauto.
+  Qed.
+
+  Lemma star_simulation:
+    forall ips t ips',
+      Star (PS.sem prog ctx) ips t ips' ->
+    forall ics,
+      PS.partial_state ctx ics ips ->
+    exists ics',
+      Star (CS.sem prog) ics t ics' /\ PS.partial_state ctx ics' ips'.
+  Proof.
+    intros ips t ips' Hstar.
+    induction Hstar; subst.
+    - eexists. split.
+      + left.
+      + auto.
+    - intros ics Hics_partial.
+      destruct (lockstep_simulation s1 t1 s2 H ics Hics_partial) as [ics' []].
+      destruct (IHHstar ics' H1) as [ics'' []].
+      exists ics''. split.
+      + eapply star_left; eauto.
+      + auto.
+  Qed.
+
+  Theorem CS_simulates_PS:
+    forward_simulation (PS.sem prog ctx) (CS.sem prog).
+  Proof.
+    eapply forward_simulation_step.
+    - apply match_initial_states.
+    - apply match_final_states.
+    - apply lockstep_simulation.
+  Qed.
+
+  Lemma context_validity:
+    forall C CI,
+      PMap.MapsTo C CI ctx -> PMap.MapsTo C CI (prog_interface prog).
+  Proof.
+    intros.
+    apply PMapFacts.empty_mapsto_iff in H.
+    contradiction.
+  Qed.
+
+  Corollary partial_semantics_implies_complete_semantics:
+    forall beh,
+      program_behaves (PS.sem prog ctx) beh ->
+      program_behaves (CS.sem prog) beh.
+  Proof.
+    intros.
+
+    (* manually prove that PS is going wrong *)
+    
+    destruct (forward_simulation_behavior_improves CS_simulates_PS H)
+      as [beh' [Hbeh []]]; subst; auto.
+
+    destruct H0 as [t []]; subst.
+
+    inversion H; subst.
+    - (* program has run *)
+      inversion H0; subst.
+      eapply program_runs.
+      + eauto.
+      + inversion H2; subst.
+        destruct (star_simulation s t s' H6 ics H3) as [? []].
+        econstructor.
+        * eauto.
+        * unfold nostep in *. intros.
+          unfold not. intro.
+          destruct (Decomposition.lockstep_simulation prog ctx x t0 s'0 H10 s' H9)
+            as [s'' []].
+          eapply H7. econstructor; eauto.
+        * unfold not. intros.
+          apply H8. econstructor; eauto.
+          ** PS.simplify_turn. unfold not. intro.
+             destruct s'. repeat destruct p. 
+             eapply PMapFacts.empty_in_iff in H11; inversion H11.
+             destruct c. destruct p.
+             eapply PMapFacts.empty_in_iff in H11; inversion H11.
+    - (* program went wrong immediately *)
+      eapply program_goes_initially_wrong.
+      intros. unfold not. intro.
+      specialize (H2 (PS.partialize s ctx)).
+      apply H2. econstructor.
+      + apply PS.partialize_correct.
+        reflexivity.
+      + auto.
+  Qed.
+End PS2CS.
+
+Section PartialComposition.
+  Variable prog1 prog2: program.
+
+  Hypothesis same_main:
+    prog_main prog1 = prog_main prog2.
+
+  Hypothesis disjointness:
+    PMapExtra.Disjoint (prog_interface prog1) (prog_interface prog2).
+
+  (* at some point we will have to use the fact that the link gives us a good program *)
+  (*
+  Hypothesis closedness:
+    closed_program (program_link prog1 prog2 (fst (prog_main prog1)) (snd (prog_main prog1))).
+*)
+
+  Let prog := program_link prog1 prog2 (fst (prog_main prog1)) (snd (prog_main prog1)).
+  Let empty_ctx := PMap.empty Component.interface.
+  Let G := init_genv prog.
+
+  Definition multi_state : Type := PS.state * PS.state.
+
+  Inductive multi_initial_state: multi_state -> Prop :=
+  | multi_initial_state_intro: forall ics ips1 ips2,
+      PS.partial_state (prog_interface prog2) ics ips1 ->
+      PS.partial_state (prog_interface prog1) ics ips2 ->
+      PS.mergeable_states ips1 ips2 ->
+      CS.initial_state prog ics ->
+      multi_initial_state (ips1, ips2).
+
+  Inductive multi_final_state : multi_state -> Prop :=
+  | multi_final_state_intro: forall ics ips1 ips2,
+      PS.partial_state (prog_interface prog2) ics ips1 ->
+      PS.partial_state (prog_interface prog1) ics ips2 ->
+      PS.mergeable_states ips1 ips2 ->
+      CS.final_state G ics ->
+      multi_final_state (ips1, ips2).
+
+  Inductive multi_step (G: global_env)
+    : multi_state -> trace -> multi_state -> Prop :=
+  | mstep: forall ips1 t ips1' ips2 ips2',
+      PS.step (prog_interface prog2) G ips1 t ips1' ->
+      PS.step (prog_interface prog1) G ips2 t ips2' ->
+      PS.mergeable_states ips1 ips2 ->
+      multi_step G (ips1, ips2) t (ips1', ips2').
+
+  Definition multisem :=
+    @Semantics_gen multi_state global_env
+                   multi_step multi_initial_state multi_final_state G.
+
+  Inductive multi_match : multi_state -> PS.state -> Prop :=
+  | mmatch_first: forall ips1 ips2,
+      PS.is_program_component ips1 (prog_interface prog2) ->
+      PS.is_context_component ips2 (prog_interface prog1) ->
+      PS.mergeable_states ips1 ips2 ->
+      multi_match (ips1, ips2) (PS.merge_partial_states ips1 ips2)
+  | mmatch_second: forall ips1 ips2,
+      PS.is_context_component ips1 (prog_interface prog2) ->
+      PS.is_program_component ips2 (prog_interface prog1) ->
+      PS.mergeable_states ips1 ips2 ->
+      multi_match (ips1, ips2) (PS.merge_partial_states ips1 ips2).
+
+  (* if ics is a partial state of ips1 and ips2 in, respectively, ctx1 and ctx2,
+     it means that it is also a partial state of the merge of ips1 and ips2 in
+     the empty context *)
+  Lemma merged_state_preserves_partiality:
+    forall ips1 ips2 ics,
+      PS.partial_state (prog_interface prog2) ics ips1 ->
+      PS.partial_state (prog_interface prog1) ics ips2 ->
+      PS.partial_state empty_ctx ics (PS.merge_partial_states ips1 ips2).
+  Proof.
+  Admitted.
+
+  Lemma partial_state_weakening:
+    forall ips1 ips2 ics,
+      PS.partial_state (prog_interface prog2) ics ips1 ->
+      PS.partial_state empty_ctx ics (PS.merge_partial_states ips1 ips2).
+  Proof.
+  Admitted.
+
+  (* after the merge, the context will never execute *)
+  Lemma merged_state_always_executes_the_program:
+    forall ips1 ips2,
+      PS.mergeable_states ips1 ips2 ->
+      PS.is_program_component (PS.merge_partial_states ips1 ips2) empty_ctx.
+  Proof.
+  Admitted.
+
+  Lemma multi_match_initial_states:
+    forall ms,
+      multi_initial_state ms ->
+    exists ips,
+      PS.initial_state prog empty_ctx ips /\ multi_match ms ips.
+  Proof.
+    intros ms Hms_init.
+    inversion Hms_init; subst.
+    exists (PS.merge_partial_states ips1 ips2). split.
+    - econstructor; eauto.
+      + eapply merged_state_preserves_partiality; eauto.
+    - (* case analysis how who has control *)
+      CS.unfold_state.
+      destruct (PMap.mem (Pointer.component pc) (prog_interface prog2)) eqn:Hcontrol;
+        [ apply PMapFacts.mem_in_iff in Hcontrol |
+          apply PMapFacts.not_mem_in_iff in Hcontrol ].
+      + apply mmatch_second; auto.
+        * inversion H; subst; inversion H; subst; PS.simplify_turn;
+            try contradiction; auto.
+        * inversion H0; subst; inversion H; subst; PS.simplify_turn; auto.
+          inversion H; subst; inversion H0; subst; PS.simplify_turn; auto.
+          exfalso.
+          apply (disjointness (Pointer.component pc)). split; auto.
+      + apply mmatch_first; auto.
+        * inversion H; subst; inversion H; subst; PS.simplify_turn;
+            try contradiction; auto.
+        * inversion H0; subst; inversion H; subst; PS.simplify_turn; auto.
+          inversion H; subst; inversion H0; subst; PS.simplify_turn; auto.
+          (* Pointer.component pc isn't in ctx1, nor it is in ctx2, that should be
+             impossible *)
+          (* notice that we know Pointer.component pc to be equal to (fst (prog_main p)) *)
+          destruct H2 as [? [? [? [Hpc []]]]].
+          (*
+          destruct closedness as [Hclosed_interface Hmain_existence].
+          destruct Hmain_existence as [mainC_procs []].
+          simpl in *.*)
+          admit.
+  Admitted.
+
+  Lemma multi_match_final_states:
+    forall ms ips,
+      multi_match ms ips ->
+      multi_final_state ms ->
+      PS.final_state prog empty_ctx ips.
+  Proof.
+    intros ms ips Hmmatch Hms_final.
+    inversion Hms_final; subst.
+    inversion Hmmatch; subst.
+    - eapply PS.final_state_program; eauto.
+      + apply merged_state_always_executes_the_program; auto.
+      + eapply merged_state_preserves_partiality; eauto.
+    - eapply PS.final_state_program; eauto.
+      + apply merged_state_always_executes_the_program; auto.
+      + eapply merged_state_preserves_partiality; eauto.
+  Qed.
+
+  Lemma threeway_simulation:
+    forall ms t ms',
+      multi_step G ms t ms' ->
+    forall ips,
+      multi_match ms ips ->
+    exists ips',
+      PS.step empty_ctx G ips t ips' /\ multi_match ms' ips'.
+  Proof.
+    intros ms t ms' Hstep.
+    intros ips Hmatch.
+
+    inversion Hstep; subst.
+
+    exists (PS.merge_partial_states ips1' ips2'). split.
+    - inversion H; subst.
+      inversion Hmatch; subst;
+        econstructor; eauto; apply partial_state_weakening; auto.
+    - (* case analysis how who has control *)
+  Admitted.
+
+  Theorem prog_simulates_prog1_and_prog2:
+    forward_simulation multisem (PS.sem prog (PMap.empty Component.interface)).
+  Proof.
+    eapply forward_simulation_step.
+    - apply multi_match_initial_states.
+    - apply multi_match_final_states.
+    - apply threeway_simulation.
+  Qed.
+
+  Corollary partial_programs_composition:
+    forall beh,
+      program_behaves (PS.sem prog1 (prog_interface prog2)) beh ->
+      program_behaves (PS.sem prog2 (prog_interface prog1)) beh ->
+      program_behaves (PS.sem prog empty_ctx) beh.
+  Proof.
+    (* this should be provable, but it might be tricky *)
+  Admitted.
+End PartialComposition.
+
+Section Composition.
+  Variable p c: program.
+
+  Let mainC := fst (prog_main p).
+  Let mainP := snd (prog_main p).
+
+  Hypothesis same_main:
+    prog_main p = prog_main c.
+
+  Hypothesis disjointness:
+    PMapExtra.Disjoint (prog_interface p) (prog_interface c).
+
+  Hypothesis closedness:
+    closed_program (program_link p c mainC mainP).
+
+  Theorem composition:
+    forall beh,
+      program_behaves (PS.sem p (prog_interface c)) beh ->
+      program_behaves (PS.sem c (prog_interface p)) beh ->
+      program_behaves (CS.sem (program_link p c mainC mainP)) beh.
+  Proof.
+    intros beh Hbeh1 Hbeh2.
+    destruct closedness.
+    eapply partial_semantics_implies_complete_semantics.
+    apply partial_programs_composition; auto.
+  Qed.
+End Composition.
