S2I/Definitions.v
@@ -21,8 +21,4 @@ Module I.
 End I.
 
 Ltac simplify_turn :=
-  unfold S.PS.is_program_component, S.PS.is_context_component in *;
-  unfold I.PS.is_program_component, I.PS.is_context_component in *;
-  unfold turn_of, S.PS.state_turn, I.PS.state_turn in *;
-  simpl in *;
-  auto.
+  S.PS.simplify_turn; I.PS.simplify_turn.
